Coc/Substitution.lean
@@ -6,7 +6,34 @@ import Coc.Defs
 namespace Coc
 section
 
+mutual
+inductive Subs where
+  | id : Subs
+  | shift : Subs
+  | cons : ES → Subs → Subs
+  | comp : Subs → Subs → Subs
 
+inductive ES where
+  | sort : Nat →       ES
+  | var  : Nat →       ES
+  | app  : ES → ES →   ES
+  | lam  : ES → ES →   ES
+  | pi   : ES → ES →   ES
+  | subs : ES → Subs → ES
+end
+
+-- TODO: mutual recursion and termination proof
+def simplify : ES → ES
+  | .subs (.sort s) _   => .sort s
+  | .subs (.var 0)        (.cons h _) => h
+  | .subs (.var (n + 1))  (.cons _ t) => simplify (.subs (.var n) t)
+  | .subs (.var n) σ    => .subs (.var n) σ -- TODO
+  | .subs (.app s t) σ  => simplify (.app (.subs s σ) (.subs t σ))
+  | .subs (.lam t e) σ  => .lam (simplify (.subs t σ)) (.subs e (.cons (.var 0) (.comp σ .shift)))
+  | .subs (.pi t₁ t₂) σ => .pi (simplify (.subs t₁ σ)) (.subs t₂ (.cons (.var 0) (.comp σ .shift)))
+  | .subs (.subs e τ) σ => simplify (.subs e (.comp τ σ))
+  | e                   => e -- TODO
+termination_by _ e => e
 
 end
 end Coc
